src/LibMap.v
@@ -58,7 +58,7 @@ Instance single_bind_inst : forall A B, BagSingleBind A B (map A B).
   constructor. rapply (@single_bind_impl A B). Defined.
 Instance binds_inst : forall A B, BagBinds A B (map A B). 
   constructor. rapply (@binds_impl A B). Defined.
-Instance union_inst : forall A B, BagUnion (map A B). (* todo: bug pas si on enlève B *)
+Instance union_inst : forall A B, BagUnion (map A B). (* todo: bug pas si on enlve B *)
   constructor. rapply (@union_impl A B). Defined.
 Instance remove_inst : forall A B, BagRemove (map A B) (set A).
   constructor. rapply (@remove_impl A B). Defined.
@@ -121,7 +121,7 @@ Lemma in_dom_empty : forall A B x,
   x \indom (\{} : map A B) ->
   False.
 Proof.
-  intros. rewrite dom_empty in *. eapply in_empty. eauto.
+  intros. rewrite dom_empty in *. eapply in_empty; typeclass.
 Qed.
 
 Lemma no_binds_empty : forall (A B : Type) (M : map A B),
@@ -143,8 +143,7 @@ Proof.
   eauto using set_in_empty_inv.
 Qed.
 
-End Properties. 
-
+End Properties.
 
 Axiom restrict_read : forall A `{Inhab B} (M:map A B) i j,
   i <> j -> (M\--i)\(j) = M\(j).
