src/open.sh
@@ -9,4 +9,5 @@ fi
 echo coqbin=${COQBIN}
 ${COQBIN}coqide -R . TLC $*
 
-#-dont-load-proofs 
+
+#-dont-load-proofs  -async-proofs-j 1
